doc/developer/semantics/Mz.lean
@@ -17,3 +17,4 @@ import Mz.Aggregate
 import Mz.Consolidate
 import Mz.Triple
 import Mz.Join
+import Mz.GroupBy
